<?xml version="1.0"?>

<!DOCTYPE uridef[
  <!ENTITY rdf 		      "http://www.w3.org/1999/02/22-rdf-syntax-ns#">
  <!ENTITY rdfs 	      "http://www.w3.org/2000/01/rdf-schema#">
  <!ENTITY owl 		      "http://www.w3.org/2002/07/owl#">
  <!ENTITY xsd 		      "http://www.w3.org/2001/XMLSchema#">
  <!ENTITY credentials 	  "http://chacs.nrl.navy.mil/projects/4SEA/NRLOntologyFiles/credentials.owl#">
  <!ENTITY algorithms 	  "http://chacs.nrl.navy.mil/projects/4SEA/NRLOntologyFiles/securityAlgorithms.owl#">
  <!ENTITY assurance 	  "http://chacs.nrl.navy.mil/projects/4SEA/NRLOntologyFiles/securityAssurance.owl#">
  <!ENTITY security 	  "http://chacs.nrl.navy.mil/projects/4SEA/NRLOntologyFiles/securityMain.owl#">
  ]>
  
<rdf:RDF
    xmlns             ="&security;"
    xmlns:security    ="&security;" 
    xml:base          ="&security;"
    xmlns:rdf         ="&rdf;"
    xmlns:rdfs        ="&rdfs;"
    xmlns:owl         ="&owl;"
    xmlns:xsd         ="&xsd;"
    xmlns:credentials ="&credentials;"
    xmlns:algorithms  ="&algorithms;"
    xmlns:assurance   ="&assurance;"
>
    
 <owl:Ontology>
   <rdfs:comment>
      A security ontology to annotate resources with security-related information
   </rdfs:comment>
 </owl:Ontology>
   
 <!-- Top Level Classes; SecurityObjective and SecurityConcept
 -->
 
  <owl:Class rdf:ID="SecurityObjective"/>
  
  <owl:Class rdf:ID="SecurityConcept">
    <owl:disjointWith rdf:resource="#SecurityObjective"/>
  </owl:Class>
  
  
 <!--
 Second Tier classes, subclasses of SecurityConcept; 
 SecurityProtocol, SecurityMechansism, SecurityPolicy 
 -->
 
  <owl:Class rdf:ID="SecurityProtocol">
    <rdfs:subClassOf rdf:resource="#SecurityConcept"/>
  </owl:Class>
  
  <owl:Class rdf:ID="SecurityMechanism">
    <rdfs:subClassOf rdf:resource="#SecurityConcept"/>
  </owl:Class>
  
  <!-- Only SecurityPolicy is disjoint with SecurityMechanism and SecurityProtocol.
       This implies that a Mechanism and Protocol are not disjoint and thus 
       can have the same instance. We are purposefully blurring this line, 
       since a protocol can also be a mechanism.
  -->
  <owl:Class rdf:ID="SecurityPolicy">
    <rdfs:subClassOf rdf:resource="#SecurityConcept"/>
    <owl:disjointWith rdf:resource="#SecurityProtocol"/>
    <owl:disjointWith rdf:resource="#SecurityMechanism"/>
    <rdfs:subClassOf>
      <owl:Restriction>
        <owl:onProperty rdf:resource="#supportsSecurityObjective"/>
        <owl:hasValue rdf:resource="#Authorization"/>
      </owl:Restriction>
    </rdfs:subClassOf>
  </owl:Class>
    
 <!-- 
 Subclasses of SecurityProtocol class, including
 SignatureProtocol, AuthenticationProtocol, NetworkSecurityProtocol, EncryptionProtocol, and KeyMgmtProtocol
 -->
 
  <owl:Class rdf:ID="AuthenticationProtocol">
    <rdfs:subClassOf rdf:resource="#SecurityProtocol"/>
    <rdfs:subClassOf>
      <owl:Restriction>
        <owl:onProperty rdf:resource="#supportsSecurityObjective"/>
        <owl:hasValue rdf:resource="#UserAuthentication"/>
      </owl:Restriction>
    </rdfs:subClassOf>
  </owl:Class> 
  
  <owl:Class rdf:ID="KeyManagementProtocol">
    <rdfs:subClassOf rdf:resource="#SecurityProtocol"/>
    <rdfs:subClassOf>
      <owl:Restriction>
        <owl:onProperty rdf:resource="#supportsSecurityObjective"/>
        <owl:hasValue rdf:resource="#KeyManagement"/>
      </owl:Restriction>
    </rdfs:subClassOf>
  </owl:Class>

  <owl:Class rdf:ID="EncryptionProtocol">
    <rdfs:subClassOf rdf:resource="#SecurityProtocol"/>
    <rdfs:subClassOf>
      <owl:Restriction>
        <owl:onProperty rdf:resource="#supportsSecurityObjective"/>
        <owl:hasValue rdf:resource="#Confidentiality"/>
      </owl:Restriction>
    </rdfs:subClassOf>
  </owl:Class>

  <owl:Class rdf:ID="SignatureProtocol">
    <rdfs:subClassOf rdf:resource="#SecurityProtocol"/>
    <rdfs:subClassOf>
      <owl:Restriction>
        <owl:onProperty rdf:resource="#supportsSecurityObjective"/>
        <owl:hasValue rdf:resource="#MessageAuthentication"/>
      </owl:Restriction>
    </rdfs:subClassOf>
  </owl:Class>

  <owl:Class rdf:ID="NetworkSecurityProtocol">
    <rdfs:subClassOf rdf:resource="#SecurityProtocol"/>
  </owl:Class>
  
  <!-- 
  Subclasses of SecurityMechanism class; Service, Host, Network, Application
  -->
  
  <owl:Class rdf:ID="ServiceMechanism">
    <rdfs:subClassOf rdf:resource="#SecurityMechanism"/>
  </owl:Class>
  
  <owl:Class rdf:ID="HostMechanism">
    <rdfs:subClassOf rdf:resource="#SecurityMechanism"/>
  </owl:Class>
  
  <owl:Class rdf:ID="NetworkMechanism">
    <rdfs:subClassOf rdf:resource="#SecurityMechanism"/>
  </owl:Class>
  
  <owl:Class rdf:ID="ApplicationMechanism">
    <rdfs:subClassOf rdf:resource="#SecurityMechanism"/>
  </owl:Class>
  
  <!-- 
  Subclasses of SecurityPolicy class; Commercial, Military
  -->
  
  <owl:Class rdf:ID="CommercialPolicy">
    <rdfs:subClassOf rdf:resource="#SecurityPolicy"/>
  </owl:Class>
  
  <owl:Class rdf:ID="MilitaryPolicy">
    <rdfs:subClassOf rdf:resource="#SecurityPolicy"/>
  </owl:Class>

  <!-- 
  Property Definitions: SecurityConcept class
  -->
  
  <owl:ObjectProperty rdf:ID="supportsSecurityObjective">
    <rdfs:domain rdf:resource="#SecurityConcept"/>
    <rdfs:range rdf:resource="#SecurityObjective"/>
    <rdfs:comment> 
      Any SecurityConcept can support one or more of the Security Objective defined in the SecurityObjective class
    </rdfs:comment>
  </owl:ObjectProperty>
  
  <!-- 
  Property Definitions: SecurityProtocol class
  -->
  <owl:ObjectProperty rdf:ID="hasAlgorithm">
    <rdfs:domain rdf:resource="#SecurityProtocol"/>
    <rdfs:range rdf:resource="&algorithms;Algorithm"/>
  </owl:ObjectProperty>
  
  <owl:ObjectProperty rdf:ID="hasAssurance">
    <rdfs:domain>
      <owl:Class>
        <owl:unionOf rdf:parseType="Collection">
          <owl:Class rdf:about="#SecurityProtocol"/>
          <owl:Class rdf:about="#SecurityMechanism"/>
        </owl:unionOf>
      </owl:Class>
    </rdfs:domain>
    <rdfs:range rdf:resource="&assurance;Assurance"/>
  </owl:ObjectProperty>
  
  <owl:ObjectProperty rdf:ID="reqCredential">
    <rdfs:domain rdf:resource="#SecurityProtocol"/>
    <rdfs:range rdf:resource="&credentials;Credential"/>
  </owl:ObjectProperty>
  
  <!-- 
  Property Definitions: SecurityMechanism class
  -->
  <!-- Property is hasAssurance, which is already declared above -->
  
  <!-- 
  Property Definitions: SignatureProtocol class
  -->
  <owl:ObjectProperty rdf:ID="hasSignatureAlgorithm">
    <rdfs:subPropertyOf rdf:resource="#hasAlgorithm"/>
    <rdfs:domain rdf:resource="#SignatureProtocol"/>
    <rdfs:range rdf:resource="&algorithms;SignatureAlgorithm"/>
  </owl:ObjectProperty>
  
  <!-- 
  Property Definitions: EncryptionProtocol class
  -->
  <owl:ObjectProperty rdf:ID="hasEncryptionAlgorithm">
    <rdfs:subPropertyOf rdf:resource="#hasAlgorithm"/>
    <rdfs:domain rdf:resource="#EncryptionProtocol"/>
    <rdfs:range rdf:resource="&algorithms;EncryptionAlgorithm"/>
  </owl:ObjectProperty>

  <!-- 
  Instance declarations for SecurityObjective class
  -->
  
  <SecurityObjective rdf:ID="Confidentiality">
    <rdfs:comment> 
      Protects against information being disclosed or revealed to unauthorized parties.
    </rdfs:comment>
  </SecurityObjective>
  
  <SecurityObjective rdf:ID="Availability">
    <rdfs:comment> 
      Provides guarantee that resource is available to authorized users at any authorized time.
    </rdfs:comment>
  </SecurityObjective>
  
  <SecurityObjective rdf:ID="UserAuthentication">
    <rdfs:comment> 
      Provides assurance of the identity of a person or entity.
    </rdfs:comment>
  </SecurityObjective>
  
  <SecurityObjective rdf:ID="MessageAuthentication">
    <rdfs:comment> 
      Provides guarantee that message came from whoever claimed to have sent it.
    </rdfs:comment>
  </SecurityObjective>
  
  <SecurityObjective rdf:ID="Authorization">
    <rdfs:comment> 
      Only authorized entities are allowed to access resources in an authorized manner. 
      (Aka Access Control). If desired, user may create instance of AccessControl as well. 
    </rdfs:comment>
  </SecurityObjective>
  
  <SecurityObjective rdf:ID="MessageIntegrity">
    <rdfs:comment>
      Data integrity or Message integrity; data cannot be changed, deleted, modified, etc by unauthorized parties.
    </rdfs:comment>
  </SecurityObjective>
  
  <SecurityObjective rdf:ID="KeyManagement">
    <rdfs:comment> 
      (SecondaryObjective) Securely manages keys for legitimate users.
    </rdfs:comment>
  </SecurityObjective>
  
  <SecurityObjective rdf:ID="ReplayPrevention">
    <rdfs:comment>
      (Secondary Objective) Protect against replay attacks
    </rdfs:comment>
  </SecurityObjective>
  
  <SecurityObjective rdf:ID="Trust">
    <rdfs:comment>
      (Secondary Objective) How to trust entity. Trust not only of identification, but statements, claims, etc.
    </rdfs:comment>
  </SecurityObjective>
  
  <SecurityObjective rdf:ID="HostTrust">
    <rdfs:comment>
     (Secondary Objective) How to trust host or platform. Is relevant to Common criteria, etc.
    </rdfs:comment>
  </SecurityObjective>
  
  <SecurityObjective rdf:ID="CovertChannelPrevention">
    <rdfs:comment> 
      (Secondary Objective) Prevent or limit the existance of covert channels
    </rdfs:comment>
  </SecurityObjective>
  
  <SecurityObjective rdf:ID="Separation">
    <rdfs:comment>
      (Secondary Objective)
    </rdfs:comment>
  </SecurityObjective>
  
  <SecurityObjective rdf:ID="TrafficHiding">
    <rdfs:comment>
      (Secondary Objective) Pad traffic with bogus data to hide traffic patterns
    </rdfs:comment>
  </SecurityObjective>
  
  <SecurityObjective rdf:ID="Anonymity">
    <rdfs:comment>
      (Secondary Objective) Provides anonymity
    </rdfs:comment>
  </SecurityObjective>
  
  <!--
  Instance declarations for AuthenticationProtocol class
  -->
  <AuthenticationProtocol rdf:ID="Kerberos"/>

  <AuthenticationProtocol rdf:ID="SAML"/>
  
  <AuthenticationProtocol rdf:ID="LoginProtocol"/>
  
  <!--
  Instance declarations for SignatureProtocol class
  -->
  <SignatureProtocol rdf:ID="XML_DSig"/>
   
  <!--
  Instance declarations for EncryptionProtocol class
  -->
  <EncryptionProtocol rdf:ID="XML_Enc"/>
  
  <!--
  Instance declarations for KeyManagementProtocol class
  -->
  
  <KeyManagementProtocol rdf:ID="XKMS"/>
  
  <!--
  Instance declarations for NetworkSecurityProtocol class
  -->
  <NetworkSecurityProtocol rdf:ID="SSH">
    <supportsSecurityObjective rdf:resource="#MessageIntegrity"/>
    <supportsSecurityObjective rdf:resource="#Confidentiality"/>
    <supportsSecurityObjective rdf:resource="#UserAuthentication"/>
    <supportsSecurityObjective rdf:resource="#MessageAuthentication"/>
    <supportsSecurityObjective rdf:resource="#KeyManagement"/>
  </NetworkSecurityProtocol>
 
  <NetworkSecurityProtocol rdf:ID="IPSec">
    <supportsSecurityObjective rdf:resource="#MessageAuthentication"/>
    <supportsSecurityObjective rdf:resource="#MessageIntegrity"/>
    <supportsSecurityObjective rdf:resource="#Confidentiality"/>
    <supportsSecurityObjective rdf:resource="#TrafficHiding"/>
    <supportsSecurityObjective rdf:resource="#KeyManagement"/>
  </NetworkSecurityProtocol>
  
  <NetworkSecurityProtocol rdf:ID="SSL">
    <owl:sameAs rdf:resource="#TLS"/>
    <supportsSecurityObjective rdf:resource="#Confidentiality"/>
    <supportsSecurityObjective rdf:resource="#UserAuthentication"/>
    <supportsSecurityObjective rdf:resource="#KeyManagement"/>
  </NetworkSecurityProtocol>
  
  <NetworkSecurityProtocol rdf:ID="TLS">
    <owl:sameAs rdf:resource="#SSL"/>
    <supportsSecurityObjective rdf:resource="#UserAuthentication"/>
    <supportsSecurityObjective rdf:resource="#Confidentiality"/>
    <supportsSecurityObjective rdf:resource="#KeyManagement"/>
  </NetworkSecurityProtocol>
  
  <!--
  Instance declarations for SecurityMechanism:ServiceMechanism class
  -->

  <ServiceMechanism  rdf:ID="SoapFirewall">
    <supportsSecurityObjective rdf:resource="#Authorization"/>
  </ServiceMechanism>
  
  <!--
  Instance declarations for SecurityMechanism:HostMechanism class
  -->
  
  <HostMechanism rdf:ID="Safehost">
    <supportsSecurityObjective rdf:resource="#HostTrust"/>
  </HostMechanism>
  
  <HostMechanism rdf:ID="VMM">
    <supportsSecurityObjective rdf:resource="#HostTrust"/>
  </HostMechanism>
  
  <!--
  Instance declarations for SecurityMechanism:NetworkMechanism class
  -->
  
  <NetworkMechanism rdf:ID="VPN">
    <supportsSecurityObjective rdf:resource="#Confidentiality"/>
    <supportsSecurityObjective rdf:resource="#Separation"/>
  </NetworkMechanism>
  
  <NetworkMechanism rdf:ID="MLSPump">
    <supportsSecurityObjective rdf:resource="#CovertChannelPrevention"/>
  </NetworkMechanism>
  
  <NetworkMechanism rdf:ID="OnionRouter">
    <supportsSecurityObjective rdf:resource="#Anonymity"/>
    <supportsSecurityObjective rdf:resource="#Confidentiality"/>
  </NetworkMechanism>
  
  <!--
  Instance declarations for SecurityPolicy class
  -->
  
  <SecurityPolicy rdf:ID="RBAC">
    <rdfs:comment>
      Role-based Access Control
    </rdfs:comment>
  </SecurityPolicy>
    
  <!--
  Instance declarations for SecurityPolicy:Commercial class
  -->
  <CommercialPolicy rdf:ID="ClarkWilson"/>
  
  <CommercialPolicy rdf:ID="ChineseWall"/>
  
  <!--
  Instance declarations for SecurityPolicy:Military class
  -->
  <MilitaryPolicy rdf:ID="BLP">
    <rdfs:comment>Bell La-Padula</rdfs:comment>
  </MilitaryPolicy>

</rdf:RDF>

